- show that statements are false
- prove that the negation of the statement is true
- To disprove a universal statement: ∀x P(x) 
	- ∃x ¬P(x) (Counter Example)
- Examples
	- ![[Attachments/Pasted image 20201013100346.png]]
		- ![[Attachments/Pasted image 20201013100429.png]]
	- ![[Attachments/Pasted image 20201013100516.png]]
- To disprove an existential statement: ∃x P(x)
	- ∀x ¬ P(x)  
- Examples
	- ![[Attachments/Pasted image 20201013100800.png]] 
- Exercises
	- ![[Attachments/Pasted image 20201013100851.png]]